compiler/core/Imp/Lang/ImpEJsonEval.v
@@ -34,13 +34,15 @@ Require Import ImpEJson.
 Section ImpEJsonEval.
   Context {foreign_ejson_model:Set}.
   Context {fejson:foreign_ejson foreign_ejson_model}.
-  Context {fejruntime:foreign_ejson_runtime}.
+  Context {foreign_ejson_runtime_op : Set}.
+  Context {fejruntime:foreign_ejson_runtime foreign_ejson_runtime_op}.
+
   (* XXX We should try and compile the hierarchy in. Currenty it is still used in cast for sub-branding check *)
   Context (h:brand_relation_t).
 
   Section EvalInstantiation.
     (* Instantiate Imp for Qcert data *)
-    Definition imp_ejson_model_normalize (c:@imp_ejson_constant foreign_ejson_model) : imp_ejson_model :=
+    Definition imp_ejson_model_normalize (c:@imp_ejson_constant foreign_ejson_model) : @imp_ejson_model foreign_ejson_model :=
       match c with
       | cejnull => ejnull
       | cejnumber f => ejnumber f
@@ -70,11 +72,11 @@ Section ImpEJsonEval.
 
     Definition imp_ejson_Z_to_data (n: Z) : @imp_ejson_model foreign_ejson_model := ejbigint n.
 
-    Definition imp_ejson_op_eval (op:imp_ejson_op) (dl:list (@imp_ejson_model foreign_ejson_model)) : option imp_ejson_model :=
+    Definition imp_ejson_op_eval (op:imp_ejson_op) (dl:list (@imp_ejson_model foreign_ejson_model)) : option (@imp_ejson_model foreign_ejson_model) :=
       ejson_op_eval op dl. (* XXX In Common.EJson.EJsonOperators *)
 
     Definition imp_ejson_runtime_eval (op:imp_ejson_runtime_op)
-               (dl:list imp_ejson_model) : option imp_ejson_model :=
+               (dl:list (@imp_ejson_model foreign_ejson_model)) : option imp_ejson_model :=
       ejson_runtime_eval h op dl. (* XXX In Common.EJson.EJsonOperators *)
   End EvalInstantiation.
 
@@ -82,8 +84,8 @@ Section ImpEJsonEval.
   Section Evaluation.
 
     (** Evaluation takes a ImpQcert expression and an environment. It
-          returns an optional value. When [None] is returned, it
-          denotes an error. An error is always propagated. *)
+        returns an optional value. When [None] is returned, it
+        denotes an error. An error is always propagated. *)
 
     Definition imp_ejson_expr_eval
                (σ:pd_jbindings) (e:imp_ejson_expr)
@@ -112,7 +114,7 @@ Section ImpEJsonEval.
            σ el.
 
     Definition imp_ejson_decls_erase
-               (σ:option (@pd_jbindings foreign_ejson_model)) (el:list (string * option imp_ejson_expr))
+               (σ:option (@pd_jbindings foreign_ejson_model)) (el:list (string * option (@imp_ejson_expr foreign_ejson_model foreign_ejson_runtime_op)))
       : option pd_jbindings
       := imp_decls_erase σ el.
 
@@ -179,8 +181,9 @@ Section Top.
   Context {fruntime:foreign_runtime}.
   Context {foreign_ejson_model:Set}.
   Context {fejson:foreign_ejson foreign_ejson_model}.
-  Context {fdatatoejson:foreign_to_ejson}.
-  Context {fejruntime:foreign_ejson_runtime}.
+  Context {foreign_ejson_runtime_op : Set}.
+  Context {fdatatoejson:foreign_to_ejson foreign_ejson_model foreign_ejson_runtime_op}.
+  Context {fejruntime:foreign_ejson_runtime foreign_ejson_runtime_op}.
   (* XXX We should try and compile the hierarchy in. Currenty it is still used in cast for sub-branding check *)
   Context (h:brand_relation_t).
   Definition imp_ejson_eval_top (cenv: bindings) (q:imp_ejson) : option data :=
